upload old files 1

Ind.lean
@@ -1,8 +1,20 @@
 import Mathlib.Data.Nat.Basic
 
-syntax (name := coinductive) "coinductive " declId bracketedBinder* (" : " term)? (ppLine "| " ident " : " term)* : command
-
 open Lean
+
+abbrev BinderIdent := TSyntax [identKind, ``Parser.Term.hole]
+instance : Coe BinderIdent (TSyntax ``binderIdent) := ⟨(⟨·⟩)⟩
+
+-- TODO: support ∀
+partial def splitDepArrows (t : Term) (args : Array (BinderIdent × Term) := #[]) : Array (BinderIdent × Term) × Term :=
+  match t with
+  | `($type → $ret)
+  | `([$type] → $ret) => splitDepArrows ret <| args.push (⟨mkHole type⟩, type)
+  | `(($arg* : $type $[$_]?) → $ret)
+  | `(⦃$arg* : $type⦄ → $ret)
+  | `({$arg* : $type} → $ret) => splitDepArrows ret <| args ++ arg.map (·, type)
+  | `([$arg : $type] → $ret) => splitDepArrows ret <| args.push (arg, type)
+  | ret => (args, ret)
 
 abbrev CommandMacroM := StateT (Array Command) MacroM
 
@@ -25,6 +37,12 @@ partial def joinArrows : List Term → Term → MacroM Term
 partial def appHead : Term → Term
   | `($fn $_) => appHead fn
   | t => t
+
+partial def appTail : Term → Array Term
+  | `($_ $args*) => args
+  | _ => #[]
+
+syntax (name := coinductive) "coinductive " declId bracketedBinder* (" : " term)? (ppLine "| " ident " : " term)* : command
 
 structure CtorView where
   id : Ident
@@ -50,7 +68,8 @@ def CoInductiveView.ofSyntax : Syntax → MacroM CoInductiveView
       params
       type := type?.getD <| ← `(Type _)
       ctors := ← (ids.zip types).mapM λ (ctorId, type) => do
-        let (argTypes, _) := splitArrows type
+        let (argTypes, retTy) := splitArrows type
+        unless (appHead retTy).raw.matchesIdent id.getId do throw <| .error retTy "unexpected return type"
         let argTypes := argTypes.map λ argType =>
           if (appHead argType).raw.matchesIdent id.getId
           then (ty, true)
@@ -60,9 +79,7 @@ def CoInductiveView.ofSyntax : Syntax → MacroM CoInductiveView
     }
   | _ => Macro.throwUnsupported
 
-@[macro «coinductive»]
-def expandCoInductive : Macro := λ stx => CommandMacroM.run do
-  let view ← CoInductiveView.ofSyntax stx
+def defineCoInductive (view : CoInductiveView) : CommandMacroM Unit := do
   let ctors := view.ctors.map (·.id)
 
   let Approx := mkIdent <| view.id.getId ++ `Approx
@@ -123,10 +140,8 @@ def expandCoInductive : Macro := λ stx => CommandMacroM.run do
     return (← `($ctor.id $binders*), ← `(.$ctor.id $args₁*), ← `(.$ctor.id $args₂.flatten*))
   let (args₁, args₂) := args.unzip
   CommandMacroM.push `(
-    @[simp]
     def $map {$view.params* α β} (f : α → β) : @$Pattern $view.params* α → @$Pattern $view.params* β
     $[| $binders => $args₁]*
-    @[simp]
     def $mapApprox {$view.params* α ℓ} (f : α → @$Approx $view.params* ℓ) : @$Pattern $view.params* α → @$Approx $view.params* ℓ.succ
     $[| $binders => $args₁]*
     theorem $mapAgree {$view.params* α ℓ₁ ℓ₂} {f : α → @$Approx $view.params* ℓ₁} {g : α → @$Approx $view.params* ℓ₂} {x} (h : ∀ x, $Agree (f x) (g x)) : $Agree ($mapApprox f x) ($mapApprox g x) :=
@@ -137,9 +152,9 @@ def expandCoInductive : Macro := λ stx => CommandMacroM.run do
   let corec := mkIdent <| view.id.getId ++ `corec
   CommandMacroM.push `(
     def $view.id.{$view.levels,*} $view.binders* := { f : ∀ ℓ, @$Approx $view.params* ℓ // ∀ ℓ, $Agree (f ℓ) (f ℓ.succ) }
-    def $corec {$view.params* α} (f : α → @$Pattern $view.params* α) (x : α) : @$view.id $view.params* where
-      val ℓ := ℓ.rec (λ _ => .«⋯») (λ _ ih x => $mapApprox ih (f x)) x
-      property ℓ := ℓ.rec (λ _ => .«⋯») (λ _ ih _ => $mapAgree ih) x
+    def $corec {$view.params* σ} (f : σ → @$Pattern $view.params* σ) (s : σ) : @$view.id $view.params* where
+      val ℓ := ℓ.rec (λ _ => .«⋯») (λ _ ih s => $mapApprox ih (f s)) s
+      property ℓ := ℓ.rec (λ _ => .«⋯») (λ _ ih _ => $mapAgree ih) s
   )
 
   let wrappers ← CommandMacroM.run do
@@ -254,11 +269,139 @@ def expandCoInductive : Macro := λ stx => CommandMacroM.run do
       $[| .$ctors $args* => $arms]*
   )
 
+  let fold := mkIdent <| view.id.getId ++ `fold
+  let (ctors', args') := (ctors, args)
+  CommandMacroM.push `(
+    def $fold {$view.params*} : @$Pattern $view.params* (@$view.id $view.params*) → @$view.id $view.params*
+    $[| .$ctors $args* => $ctors' $args'*]*
+  )
+
   let unfold := mkIdent <| view.id.getId ++ `unfold
+  let unfold_fold := mkIdent <| unfold.getId ++ `fold
+  let fold_unfold := mkIdent <| fold.getId ++ `unfold
+  let unfold_inj := mkIdent <| unfold.getId ++ `inj
+  let unfold_corec := mkIdent <| unfold.getId ++ `corec
+  let args ← view.ctors.mapM λ ctor => do
+    let args ← ctor.argTypes.mapM λ _ => return mkIdent <| ← Elab.Term.mkFreshBinderName
+    `(λ $args* => rfl)
   CommandMacroM.push `(
     def $unfold {$view.params*} : @$view.id $view.params* → @$Pattern $view.params* (@$view.id $view.params*) :=
       $cases $(← ctors.mapM λ ctor => `(.$ctor))*
+    @[simp]
+    theorem $unfold_fold {$view.params*} : ∀ x, @$unfold $view.params* (@$fold $view.params* x) = x
+    $[| .$ctors .. => rfl]*
+    @[simp]
+    theorem $fold_unfold {$view.params*} : ∀ x, @$fold $view.params* (@$unfold $view.params* x) = x :=
+      @$cases $view.params* _ $args*
+    theorem $unfold_inj {$view.params* x y} (h : @$unfold $view.params* x = @$unfold $view.params* y) : x = y :=
+      @$fold_unfold $view.params* x ▸ @$fold_unfold $view.params* y ▸ congrArg (@$fold $view.params*) h
+    @[simp]
+    theorem $unfold_corec {$view.params* σ} f u : @$unfold $view.params* (@$corec $view.params* σ f u) = (f u).map (@$corec $view.params* σ f) := by
+      cases h : f u
+      all_goals
+        dsimp only [$map:ident, $mapApprox:ident, $unfold:ident, $cases:ident, $corec:ident]
+        try split <;> rename_i h' <;> cases h ▸ h'
+        refine (eq_rec_constant ..).trans ?_
+        congr
+      all_goals simp [h]
+      all_goals
+        funext ℓ
+        split <;> rename_i h' <;> cases h ▸ h'
+        rfl
   )
+
+  let theorems ← CommandMacroM.run do
+    for ctor in view.ctors do
+      let args ← ctor.argTypes.mapM λ _ => return mkIdent <| ← Elab.Term.mkFreshBinderName
+      CommandMacroM.push `(
+        @[simp]
+        theorem $ctor.id {$view.params*} {motive} $ctors* $args* : @$cases $view.params* motive $ctors* (.$ctor.id $args*) = $ctor.id $args* := rfl
+      )
+  CommandMacroM.push `(
+    namespace $cases
+    $theorems
+    end $cases
+  )
+
+  let theorems ← CommandMacroM.run do
+    for ctor in view.ctors do
+      let args ← ctor.argTypes.mapM λ _ => return mkIdent <| ← Elab.Term.mkFreshBinderName
+      CommandMacroM.push `(
+        @[simp]
+        theorem $ctor.id {$view.params*} $args* : @$unfold $view.params* ($ctor.id $args*) = .$ctor.id $args* := rfl
+      )
+  CommandMacroM.push `(
+    namespace $unfold
+    $theorems
+    end $unfold
+  )
+
+  let codef := mkIdent <| view.id.getId ++ `codef
+  CommandMacroM.push `(
+    def $codef {$view.params* σ} (f : σ → @$Pattern $view.params* (σ ⊕ @$view.id $view.params*) ⊕ @$view.id $view.params*) (s : σ) : @$view.id $view.params* :=
+      @$corec $view.params* (σ ⊕ @$view.id $view.params*) (λ
+        | .inl s =>
+          match f s with
+          | .inl x => x
+          | .inr x => x.unfold.map .inr
+        | .inr x => x.unfold.map .inr
+      ) (.inl s)
+  )
+
+  let unfold_codef := mkIdent <| unfold.getId ++ `codef
+  CommandMacroM.push `(
+    @[simp]
+    theorem $unfold_codef {$view.params* σ} f s : @$unfold $view.params* (@$codef $view.params* σ f s) =
+      match f s with
+      | .inl x =>
+        x.map λ
+          | .inl s => @$codef $view.params* σ f s
+          | .inr x => x
+      | .inr x => x.unfold
+    := by
+      have : ∀ x, @$corec $view.params* (σ ⊕ @$view.id $view.params*)
+        (λ | .inl s =>
+             match f s with
+             | .inl x => x
+             | .inr x => x.unfold.map .inr
+           | .inr x => x.unfold.map .inr)
+        (.inr x) = x
+      := by
+        intro x
+        apply Subtype.eq
+        funext ℓ
+        dsimp [$corec:ident]
+        induction ℓ generalizing x with
+        | zero => cases x.val .zero; rfl
+        | succ ℓ ih =>
+          dsimp
+          cases h : @$unfold $view.params* x
+          all_goals
+            rw [$map:ident, $mapApprox:ident]
+            simp [ih]
+            exact @$fold_unfold $view.params* x ▸ congrArg (@$fold $view.params*) h ▸ rfl
+      rw [$codef:ident]
+      simp
+      cases f s with
+      | inl =>
+        congr
+        funext x
+        cases x with
+        | inl => rfl
+        | inr x => exact this x
+      | inr x =>
+        dsimp
+        generalize @$unfold $view.params* x = x
+        cases x
+        all_goals
+          dsimp [$map:ident]
+          congr
+        all_goals
+          apply this
+  )
+
+def defineCoInductiveImpl (view : CoInductiveView) : CommandMacroM Unit := do
+  let ctors := view.ctors.map (·.id)
 
   let Impl := mkIdent <| view.id.getId ++ `Impl
   let Impl' := mkIdent <| view.id.getId ++ `Impl'
@@ -273,7 +416,13 @@ def expandCoInductive : Macro := λ stx => CommandMacroM.run do
     unsafe def $Impl.{$view.levels,*} $view.binders* := Thunk (@$Impl' $view.params*)
   )
 
-  let Impl_corec := mkIdent <| Impl.getId ++ `corec
+  let Pattern := mkIdent <| Impl.getId ++ `Pattern
+  let orig_Pattern := mkIdent <| view.id.getId ++ `Pattern
+  CommandMacroM.push `(
+    def $Pattern := @$orig_Pattern
+  )
+
+  let corec := mkIdent <| Impl.getId ++ `corec
   let (binders, args) := Array.unzip <| ← view.ctors.mapM λ ctor => do
     let (binders, args) := Array.unzip <| ← ctor.argTypes.mapM λ
       | (_, false) => do
@@ -281,11 +430,11 @@ def expandCoInductive : Macro := λ stx => CommandMacroM.run do
         return (x, x)
       | (_, true) => do
         let x := mkIdent <| ← Elab.Term.mkFreshBinderName
-        return (x, ← `($Impl_corec f $x))
+        return (x, ← `($corec f $x))
     return (binders, ← `(.$ctor.id $args*))
   CommandMacroM.push `(
-    unsafe def $Impl_corec {$view.params* α} (f : α → @$Pattern $view.params* α) (x : α) : @$Impl $view.params* := .mk λ _ =>
-      match f x with
+    unsafe def $corec {$view.params* σ} (f : σ → @$Pattern $view.params* σ) (s : σ) : @$Impl $view.params* := Thunk.mk λ _ =>
+      match f s with
       $[| .$ctors $binders* => $args]*
   )
 
@@ -297,7 +446,7 @@ def expandCoInductive : Macro := λ stx => CommandMacroM.run do
       let type ← joinArrows types.toList <| ← `(@$Impl $view.params*)
       CommandMacroM.push `(
         unsafe def $ctor.id {$view.params*} : $type := λ $args:ident* =>
-          .pure (.$ctor.id $args*)
+          Thunk.pure (.$ctor.id $args*)
       )
   CommandMacroM.push `(
     namespace $Impl
@@ -305,99 +454,63 @@ def expandCoInductive : Macro := λ stx => CommandMacroM.run do
     end $Impl
   )
 
-  let Impl_cases := mkIdent <| Impl.getId ++ `cases
+  let cases := mkIdent <| Impl.getId ++ `cases
   let (args, minors) := Array.unzip <| ← view.ctors.mapM λ ctor => do
     let args ← ctor.argTypes.mapM λ _ => return mkIdent <| ← Elab.Term.mkFreshBinderName
     return (args, ← `(Parser.Term.bracketedBinderF| ($ctor.id : ∀ $args:ident*, motive ($ctor.id $args*))))
   let (ctors', args') := (ctors, args)
   CommandMacroM.push `(
     @[elab_as_elim]
-    unsafe def $Impl_cases.{u} {$view.params*} {motive : @$Impl $view.params* → Sort u} $minors* x : motive x :=
-      (id rfl : .pure x.get = x) ▸
-      match x.get with
+    unsafe def $cases.{u} {$view.params*} {motive : @$Impl $view.params* → Sort u} $minors* x : motive x :=
+      (id rfl : Thunk.pure (Thunk.get x) = x) ▸
+      match Thunk.get x with
       $[| .$ctors $args* => $ctors' $args'*]*
   )
 
-  let Impl_unfold := mkIdent <| Impl.getId ++ `unfold
+  let fold := mkIdent <| Impl.getId ++ `fold
   CommandMacroM.push `(
-    unsafe def $Impl_unfold {$view.params*} : @$Impl $view.params* → @$Pattern $view.params* (@$Impl $view.params*) :=
-      $Impl_cases $(← ctors.mapM λ ctor => `(.$ctor))*
+    unsafe def $fold {$view.params*} : @$Pattern $view.params* (@$Impl $view.params*) → @$Impl $view.params*
+    $[| .$ctors $args* => $ctors' $args'*]*
   )
+
+  let unfold := mkIdent <| Impl.getId ++ `unfold
+  CommandMacroM.push `(
+    unsafe def $unfold {$view.params*} : @$Impl $view.params* → @$Pattern $view.params* (@$Impl $view.params*) :=
+      $cases $(← ctors.mapM λ ctor => `(.$ctor))*
+  )
+
+  let codef := mkIdent <| Impl.getId ++ `codef
+  let (binders, args) := Array.unzip <| ← view.ctors.mapM λ ctor => do
+    let (binders, args) := Array.unzip <| ← ctor.argTypes.mapM λ
+      | (_, false) => do
+        let x := mkIdent <| ← Elab.Term.mkFreshBinderName
+        return (x, x)
+      | (_, true) => do
+        let x := mkIdent <| ← Elab.Term.mkFreshBinderName
+        return (x, ← `($(x).casesOn ($codef f) id))
+    return (binders, ← `(.$ctor.id $args*))
+  CommandMacroM.push `(
+    unsafe def $codef {$view.params* σ} (f : σ → @$Pattern $view.params* (σ ⊕ @$Impl $view.params*) ⊕ @$Impl $view.params*) (s : σ) : @$Impl $view.params* := Thunk.mk λ _ =>
+      match f s with
+      | .inl x =>
+        match x with
+        $[| .$ctors $binders* => $args]*
+      | .inr x => Thunk.get x
+  )
+
+@[macro «coinductive»]
+def expandCoInductive : Macro := λ stx => CommandMacroM.run do
+  let view ← CoInductiveView.ofSyntax stx
+  defineCoInductive view
+  defineCoInductiveImpl view
 
 coinductive CoNat
   | zero : CoNat
   | succ : CoNat → CoNat
 
 coinductive CoList (α : Type u)
-  | nil : CoList
-  | cons : α → CoList → CoList
-
-@[simp]
-theorem CoNat.cases_zero zero succ : @cases motive zero succ .zero = zero := rfl
-
-@[simp]
-theorem CoNat.cases_succ zero succ n : @cases motive zero succ (.succ n) = succ n := rfl
-
-@[simp]
-theorem CoNat.unfold_zero : unfold zero = .zero := rfl
-
-@[simp]
-theorem CoNat.unfold_succ n : unfold (succ n) = .succ n := rfl
-
-theorem CoNat.succ.inj (h : succ n = succ n') : n = n' :=
-  Subtype.eq <| funext λ ℓ => Approx.succ.inj <| congrArg (·.val ℓ.succ) h
-
-@[simp]
-theorem CoList.cases_nil nil cons : @cases α motive nil cons .nil = nil := rfl
-
-@[simp]
-theorem CoList.cases_cons nil cons x xs : @cases α motive nil cons (.cons x xs) = cons x xs := rfl
-
-@[simp]
-theorem CoList.unfold_nil : @unfold α nil = .nil := rfl
-
-@[simp]
-theorem CoList.unfold_cons x xs : @unfold α (cons x xs) = .cons x xs := rfl
-
-theorem CoList.cons.inj (h : cons x xs = cons x' xs') : x = x' ∧ xs = xs' :=
-  have := λ ℓ : Nat => Approx.cons.inj <| congrArg (·.val ℓ.succ) h
-  ⟨this .zero |>.left, Subtype.eq <| funext (this · |>.right)⟩
-
-@[simp]
-theorem CoNat.unfold_corec f x : unfold (@corec α f x) = (f x).map (corec f) := by
-  unfold Pattern.map
-  split <;> rename_i h
-    <;> simp [unfold, cases, corec]
-    <;> split <;> rename_i h' <;> cases h ▸ h'
-    <;> congr
-  funext ℓ
-  split <;> rename_i h' <;> cases h ▸ h'
-  rfl
-
-@[simp]
-theorem CoList.unfold_corec : unfold (corec f x) = (f x).map (corec f) := by
-  unfold Pattern.map
-  split <;> rename_i h
-    <;> simp [unfold, cases, corec]
-    <;> split <;> rename_i h' <;> cases h ▸ h'
-    <;> congr
-  funext ℓ
-  split <;> rename_i h' <;> cases h ▸ h'
-  rfl
-
-theorem dcongrArg.{u, v} {α : Sort u} {β : α → Sort v} {a₁ a₂ : α} (f : ∀ x, β x) (h : a₁ = a₂) : HEq (f a₁) (f a₂) :=
-  by cases h; rfl
-
-theorem CoNat.cases_corec zero succ f x : @cases motive zero succ (@corec α f x) = match h : f x with | .zero => (Subtype.eq <| funext λ | .zero => rfl | .succ ℓ => by simp [corec, h, CoNat.zero] : corec f x = .zero) ▸ zero | .succ x' => (Subtype.eq <| funext λ | .zero => rfl | .succ ℓ => by simp [corec, h, CoNat.succ]: corec f x = .succ (corec f x')) ▸ succ (corec f x') := by
-  split
-    <;> rename_i h
-    <;> simp [cases, corec]
-    <;> split <;> rename_i h' <;> cases h ▸ h'
-  . rfl
-  . rename_i x'
-    generalize hA : succ _ = A
-    generalize hB : succ _ = B
-    sorry
+  | nil : CoList α
+  | cons : α → CoList α → CoList α
 
 def CoNat.ofNat₁ : Nat → CoNat
   | .zero => .zero
@@ -474,8 +587,56 @@ theorem CoNat.add_ofNat₂ : add (ofNat₂ a) (ofNat₂ b) = ofNat₂ (a + b) :=
   | succ b ih =>
     sorry
 
+open TSyntax.Compat in
+variable (n : Name) in
+partial def replaceGuardedCalls (ctx : Bool) : Syntax → MacroM (Bool × Syntax)
+  | `($f $as*) => do
+    let (bf, f) ← replaceGuardedCalls ctx f
+    let (bas, as) := Array.unzip <| ← as.mapM <| replaceGuardedCalls true
+    if f.isIdent && f.getId.isSuffixOf n then
+      if bas.any id then throw <| .error f "nested recursive unsupported"
+      unless ctx do throw <| .error f "unguarded recursive call"
+      return (true, ← `(.inl ⟨$as,*, ()⟩))
+    if bas.any id then
+      unless f.isIdent do throw <| .error f "not a constructor"
+      let f := mkIdent f.getId.getString
+      return (bf, ← `(.inl (.$f $as*)))
+    return (bf, ← `($f $as*))
+  | `(($t)) => do
+    let (bt, t) ← replaceGuardedCalls ctx t
+    return (bt, ← `(($t)))
+  | stx =>
+    match stx with
+    | .node info kind args => return (false, .node info kind <| ← args.mapM λ arg => return (← replaceGuardedCalls false arg).snd)
+    | stx => return (false, stx)
+
+def matchAlts := Lean.Parser.Term.matchAlts
+
+syntax (Parser.Command.unsafe)? "codef " ident bracketedBinder* " : " term matchAlts : command
+
+macro_rules
+  | `($[$safety:unsafe]? codef $n $b* : $t $[| $l,* => $rs]*) => do
+    let (args, retTy) := splitDepArrows t
+    let Pattern ← `($(mkIdent <| (appHead retTy).raw.getId ++ `Pattern) $(appTail retTy)*)
+    let (args, tys) := args.unzip
+    let ty ← `(Σ' $[($args : $tys)]*, Unit)
+    let rs' : Array Term ← rs.mapM λ r => return ⟨(← replaceGuardedCalls n.getId false r.raw).snd⟩
+    let xs ← args.mapM λ _ => return mkIdent <| ← Elab.Term.mkFreshBinderName
+    `($[$safety:unsafe]? def $n $b* : $t := @λ $xs* =>
+        have : Coe $retTy ($ty ⊕ $retTy) := ⟨.inr⟩
+        have : Coe $retTy ($Pattern ($ty ⊕ $retTy) ⊕ $retTy) := ⟨.inr⟩
+        .codef (λ ⟨$xs,*, _⟩ => match $[$xs:ident],* with $[| $l,* => $rs']*) (⟨$xs,*, ()⟩ : $ty))
+
+-- TODO: generated codef def lemma
+
 coinductive Stream'
   | cons : Nat → Stream' → Stream'
+
+def cases {motive : Thunk (α ⊕ β) → Sort u} (inl : ∀ x, motive (.pure (.inl x))) (inr : ∀ y, motive (.pure (.inr y))) t : motive t :=
+  (id rfl : .pure t.get = t) ▸
+  match t.get with
+  | .inl x => inl x
+  | .inr x => inr x
 
 def Stream'.nth (n : Nat) (s : Stream') : Nat :=
   let ⟨hd, tl⟩ := s.unfold
@@ -483,18 +644,109 @@ def Stream'.nth (n : Nat) (s : Stream') : Nat :=
   | .zero => hd
   | .succ n => nth n tl
 
-def fib : Stream' :=
-  .corec (λ (a, b) => ⟨dbgTraceVal a, (b, a + b)⟩) (0, 1)
-
-#eval fib.nth 6
-
 unsafe def Stream'.Impl.nth (n : Nat) (s : Stream'.Impl) : Nat :=
   let ⟨hd, tl⟩ := s.unfold
   match n with
   | .zero => hd
   | .succ n => nth n tl
 
-unsafe def fib' : Stream'.Impl :=
-  .corec (λ (a, b) => ⟨dbgTraceVal a, (b, a + b)⟩) (0, 1)
+codef fib : Nat → Nat → Stream'
+  | a, b => Stream'.cons (dbgTraceVal a) (fib b (a + b))
 
-#eval fib'.nth 6
+#eval (fib 0 1).nth 6
+
+unsafe codef fib' : Nat → Nat → Stream'.Impl
+  | a, b => Stream'.Impl.cons (dbgTraceVal a) (fib' b (a + b))
+
+#eval (fib' 0 1).nth 6
+
+theorem fib_def a b : fib a b = match a, b with | a, b => Stream'.cons a (fib b (a + b)) := by
+  apply Stream'.unfold.inj
+  rw [fib, Stream'.unfold.codef]
+  rfl
+
+codef count : Nat → Stream'
+  | n => Stream'.cons n (count n.succ)
+
+theorem count_def : count n = .cons n (count n.succ) :=
+  Stream'.unfold.inj <| by rw [count]; apply Stream'.unfold.codef
+
+coinductive Partial (α : Type u) : Type u
+  | pure : α → Partial α
+  | delay : Partial α → Partial α
+
+coinductive Tree (α : Type u) : Type u
+  | leaf : Tree α
+  | node : α → Tree α → Tree α → Tree α
+  | node' : Tree α → Tree α → Tree α
+
+codef Partial.bind (f : α → Partial β) : Partial α → Partial β
+  | x =>
+    match x.unfold with
+    | .pure x => f x
+    | .delay x => delay (bind x)
+
+theorem Partial.bind.def (f : α → Partial β) x : bind f x = match x with | x => match x.unfold with | .pure x => f x | .delay x => delay (bind f x) := by
+  apply unfold.inj
+  rw [bind, unfold.codef]
+  dsimp
+  cases unfold x
+  all_goals rfl
+
+instance : Monad Partial where
+  pure := .pure
+  bind x := x.bind
+
+codef Tree.ofCoList : CoList α → Tree α
+  | x =>
+    match x.unfold with
+    | .nil => @node' α leaf leaf
+    | .cons hd tl => node hd (@leaf α) (ofCoList tl)
+
+example : Partial.pure x >>= f = f x := by
+  dsimp [pure, bind]
+  rw [Partial.bind.def]
+  rfl
+
+example : Partial.delay x >>= f = Partial.delay (x >>= f) := by
+  dsimp [pure, bind]
+  rw [Partial.bind.def]
+  rfl
+
+instance : LawfulMonad Partial where
+  map_const := rfl
+  id_map x := by
+    apply Subtype.eq
+    funext ℓ
+    simp [Functor.map, Partial.corec]
+    induction ℓ generalizing x with
+    | zero => cases x.val 0; simp
+    | succ ℓ ih =>
+      simp
+      split
+      next h =>
+        simp [Partial.cases] at h
+        split at h
+        . cases h
+        . cases h
+      next A x' h =>
+        clear A
+        cases x' with
+        | inl x' =>
+          simp [ih]
+          sorry
+        | inr x' =>
+          simp
+          sorry
+  seqLeft_eq _ _ := sorry
+  seqRight_eq _ _ := sorry
+  pure_seq _ _ := sorry
+  bind_pure_comp _ _ := rfl
+  bind_map _ _ := rfl
+  pure_bind x f := by
+    dsimp only [pure, bind]
+    rw [Partial.corec'_yield]
+    dsimp
+  bind_assoc _ _ _ := sorry
+
+--#check Partial.corec
