Strict.lean
@@ -6,9 +6,9 @@ unsafe inductive A
 unsafe def A.intro.inj : intro x = intro y → x = y :=
   @Eq.rec A (intro x) (rec λ y _ => x = y) rfl (intro y)
 
-unsafe def f : (A → Prop) → A := (⟨Eq ·⟩)
+unsafe def f (s : Set A) : A := ⟨Set.singleton s⟩
 
 unsafe def f.inj (h : f x = f y) : x = y :=
-  congrFun (A.intro.inj h) y ▸ rfl
+  cast (congrFun (A.intro.inj h) x) rfl
 
-#check Function.cantor_injective f @f.inj
+unsafe def False.intro := Function.cantor_injective f @f.inj
