FreeMonad.lean
@@ -1,0 +1,332 @@
+namespace Quot
+
+variable {α : Sort u} {r : α → α → Prop} {β : Sort v} {γ : Sort w} (f : (β → α) → γ)
+
+private unsafe def liftF.impl (_ : ∀ a b, (∀ x, mk r (a x) = mk r (b x)) → f a = f b) (q : β → Quot r) : γ :=
+  f λ x => unsafeCast <| q x
+
+@[implemented_by liftF.impl]
+def liftF (c : ∀ a b, (∀ x, mk r (a x) = mk r (b x)) → f a = f b) (q : β → Quot r) : γ :=
+  f λ x => Classical.choose (q x).exists_rep
+
+theorem liftF_mk (c : ∀ a b, (∀ x, mk r (a x) = mk r (b x)) → f a = f b) (a : β → α) : liftF f c (λ x => mk r (a x)) = f a :=
+  c _ a λ _ => Classical.choose_spec <| exists_rep _
+
+end Quot
+
+namespace Quotient
+
+variable {α : Sort u} {s : Setoid α} {β : Sort v} {γ : Sort w} (f : (β → α) → γ) (c : ∀ a b, (∀ x, a x ≈ b x) → f a = f b)
+
+def liftF (q : β → Quotient s) : γ :=
+  Quot.liftF f (λ a b h => c a b λ x => exact <| h x) q
+
+theorem liftF_mk (a : β → α) : Quotient.liftF f c (λ x => .mk s (a x)) = f a :=
+  Quot.liftF_mk ..
+
+end Quotient
+
+set_option autoImplicit false
+
+universe u
+
+inductive FreeStateM (σ α : Type u) : Type u
+  | pure (a : α)
+  | get (k : σ → FreeStateM σ α)
+  | set (s : σ) (k : FreeStateM σ α)
+
+variable {σ α : Type u}
+
+inductive FreeStateM.Eq : FreeStateM σ α → FreeStateM σ α → Prop
+  | pure a : Eq (pure a) (pure a)
+  | get {k₁ k₂} : (∀ s, Eq (k₁ s) (k₂ s)) → Eq (get k₁) (get k₂)
+  | set {k₁ k₂} s : Eq k₁ k₂ → Eq (set s k₁) (set s k₂)
+
+  | symm {k₁ k₂} : Eq k₁ k₂ → Eq k₂ k₁
+  | trans {k₁ k₂ k₃} : Eq k₁ k₂ → Eq k₂ k₃ → Eq k₁ k₃
+
+  | get_get (k : _ → _) : Eq (get (λ s => get (k s))) (get (λ s => k s s))
+  | get_set k : Eq (get λ s => set s k) k
+  | set_get s k : Eq (set s (get k)) (set s (k s))
+  | set_set s₁ s₂ k : Eq (set s₁ (set s₂ k)) (set s₂ k)
+
+theorem FreeStateM.Eq.refl : (k : FreeStateM σ α) → Eq k k
+  | .pure a => pure a
+  | .get k => get λ s => refl (k s)
+  | .set s k => set s <| refl k
+
+def StateM' (σ α : Type u) := Quotient ⟨@FreeStateM.Eq σ α, .refl, .symm, .trans⟩
+
+def StateM'.pure (a : α) : StateM' σ α :=
+  .mk _ <| .pure a
+
+def StateM'.get : (k : σ → StateM' σ α) → StateM' σ α :=
+  .liftF (λ k => .mk _ <| .get k) λ _ _ hk => Quot.sound <| .get hk
+
+def StateM'.set (s : σ) : (k : StateM' σ α) → StateM' σ α :=
+  .lift (λ k => .mk _ <| .set s k) λ _ _ hk => Quot.sound <| .set s hk
+
+def StateM'.bind' {β : Type u} (f : α → StateM' σ β) : (k : FreeStateM σ α) → StateM' σ β
+  | .pure a => f a
+  | .get k => .get λ s => bind' f (k s)
+  | .set s k => .set s (bind' f k)
+
+theorem StateM'.bind_wf {β} f k₁ k₂ (hk : FreeStateM.Eq k₁ k₂) : @bind' σ α β f k₁ = bind' f k₂ := by
+  induction hk with dsimp [bind']
+  | get _ ih => congr; exact funext ih
+  | set => congr
+  | symm _ ih => exact ih.symm
+  | trans _ _ ih₁ ih₂ => exact ih₁.trans ih₂
+  | get_get k =>
+    refine .trans (Quotient.liftF_mk ..) ?_
+    apply Quot.sound
+    exact .get_get ..
+  | get_set k =>
+    cases bind' f k using Quot.ind with
+    | mk =>
+      apply Quot.sound
+      refine .trans ?_ <| .get_set _
+      refine .get ?_
+      intro s
+      apply Quotient.exact (s := ⟨_, _⟩)
+      exact Classical.choose_spec <| Quot.exists_rep _
+  | set_get s k =>
+    cases h : bind' f (k s) using Quot.ind with
+    | mk =>
+      apply Quot.sound
+      refine .trans (.set_get ..) ?_
+      refine .set _ ?_
+      apply Quotient.exact (s := ⟨_, _⟩)
+      refine .trans ?_ h
+      exact Classical.choose_spec <| Quot.exists_rep _
+  | set_set s₁ s₂ k =>
+    cases bind' f k using Quot.ind with
+    | mk =>
+      apply Quot.sound
+      exact .set_set ..
+
+def StateM'.bind {β : Type u} (f : α → StateM' σ β) : (k : StateM' σ α) → StateM' σ β :=
+  .lift (bind' f) (bind_wf f)
+
+instance : Monad (StateM' σ) where
+  pure := .pure
+  bind k := k.bind
+
+@[simp]
+theorem StateM'.bind_pure {β} f a : @bind σ α β f (pure a) = f a := rfl
+
+@[simp]
+theorem StateM'.bind_get {β} f k : @bind σ α β f (get k) = get λ s => bind f (k s) := by
+  refine Quot.sound <| .get λ s => ?_
+  apply Quotient.exact (s := ⟨_, _⟩)
+  generalize h : k s = x
+  have h₁ : ∃ a, _ = k s := Quot.exists_rep _
+  have h₂ : ∃ a, _ = bind' f (Classical.choose h₁) := Quot.exists_rep _
+  have h₃ : ∃ a, _ = bind f (k s) := Quot.exists_rep _
+  cases x using Quot.ind with
+  | mk x =>
+    show Quot.mk _ (Classical.choose h₂) = Quot.mk _ (Classical.choose h₃)
+    apply Eq.trans <| Classical.choose_spec h₂
+    apply Eq.trans <| bind_wf f _ x <| Quotient.exact <| Classical.choose_spec h₁ |>.trans h
+    apply Eq.trans _ <| .symm <| Classical.choose_spec h₃
+    exact .symm <| congrArg _ h
+
+@[simp]
+theorem StateM'.bind_set {β} f s k : @bind σ α β f (set s k) = set s (bind f k) := by
+  cases k using Quot.ind with
+  | mk => rfl
+
+@[eliminator]
+def StateM'.ind {motive : StateM' σ α → Prop}
+  (pure : ∀ a, motive (pure a))
+  (get : ∀ k, (∀ s, motive (k s)) → motive (get k))
+  (set : ∀ s k, motive k → motive (set s k))
+  t : motive t := by
+  cases t using Quot.ind with
+  | mk t =>
+    induction t with
+    | pure a => exact pure a
+    | get _ ih =>
+      specialize get _ ih
+      conv at get => arg 1; apply Quotient.liftF_mk
+      exact get
+    | set s _ ih => exact set s _ ih
+
+instance : LawfulMonad (StateM' σ) where
+  map_const := rfl
+  id_map x := by
+    dsimp [Functor.map]
+    induction x with simp <;> congr
+    | get _ ih => exact funext ih
+  seqLeft_eq x y := by
+    dsimp [SeqLeft.seqLeft, Seq.seq, Functor.map]
+    induction x with simp <;> congr
+    | get _ ih => exact funext ih
+  seqRight_eq x y := by
+    dsimp [SeqRight.seqRight, Seq.seq, Functor.map]
+    induction x with simp <;> congr
+    | pure =>
+      induction y with simp <;> congr
+      | get _ ih => exact funext ih
+    | get _ ih => exact funext ih
+  pure_seq _ _ := rfl
+  bind_pure_comp _ _ := rfl
+  bind_map _ _ := rfl
+  pure_bind _ _ := rfl
+  bind_assoc x _ _ := by
+    dsimp [bind]
+    induction x with simp <;> congr
+    | get _ ih => exact funext ih
+
+instance : MonadState σ (StateM' σ) where
+  get := .get .pure
+  set s := .set s (.pure .unit)
+  modifyGet f := .get λ s => let (a, s) := f s; .set s (.pure a)
+
+def StateM'.toStateM' : FreeStateM σ α → StateM σ α
+  | .pure a => StateT.pure a
+  | .get k => StateT.get.bind λ s => toStateM' <| k s
+  | .set s k => StateT.set s |>.bind λ _ => toStateM' k
+
+theorem StateM'.toStateM_wf (k₁ k₂ : FreeStateM σ α) (hk : FreeStateM.Eq k₁ k₂) : toStateM' k₁ = toStateM' k₂ := by
+  induction hk with dsimp [toStateM', StateT.bind, StateT.get, StateT.set]
+  | get _ ih => exact funext λ s => congrFun (ih s) s
+  | set s _ ih => exact funext λ _ => congrFun ih s
+  | symm _ ih => exact ih.symm
+  | trans _ _ ih₁ ih₂ => exact ih₁.trans ih₂
+
+def StateM'.ofStateM : StateM σ α → StateM' σ α := modifyGet
+def StateM'.toStateM : StateM' σ α → StateM σ α := Quot.lift toStateM' toStateM_wf
+
+@[simp]
+theorem StateM'.toStateM_pure a : @toStateM σ α (pure a) = StateT.pure a := rfl
+
+@[simp]
+theorem StateM'.toStateM_get k : @toStateM σ α (get k) = StateT.get.bind λ s => toStateM (k s) := by
+  funext s
+  generalize h : k s = x
+  cases x using Quot.ind with
+  | mk x =>
+    show toStateM' (Classical.choose _) s = toStateM _ _
+    apply Eq.trans
+    . apply congrFun (f := toStateM' <| Classical.choose _)
+      apply toStateM_wf _ x
+      apply Quotient.exact (s := ⟨_, _⟩)
+      apply Eq.trans _ h
+      exact Classical.choose_spec <| Quot.exists_rep _
+    rw [h]
+    rfl
+
+@[simp]
+theorem StateM'.toStateM_set s k : @toStateM σ α (set s k) = (StateT.set s).bind λ _ => toStateM k := by
+  cases k using Quot.ind with
+  | mk k => rfl
+
+theorem StateM'.toStateM_ofStateM (k : StateM σ α) : toStateM (ofStateM k) = k := by
+  funext s
+  show toStateM' (Classical.choose _) s = _
+  apply congrFun (g := λ _ => k s)
+  apply toStateM_wf _ <| .set _ <| .pure _
+  apply Quotient.exact (s := ⟨_, _⟩)
+  exact Classical.choose_spec <| Quot.exists_rep _
+
+theorem StateM'.ofStateM_toStateM (k : StateM' σ α) : ofStateM (toStateM k) = k := by
+  dsimp [ofStateM, modifyGet]
+  apply Eq.trans <| Quotient.liftF_mk ..
+  cases k using Quot.ind with
+  | mk k =>
+    apply Quot.sound
+    dsimp [toStateM]
+    induction k with dsimp [toStateM', StateT.pure, StateT.bind, StateT.get, StateT.set]
+    | pure => exact .get_set _
+    | get k ih =>
+      refine .trans ?_ <| .get ih
+      clear ih
+      refine .trans ?_ <| .symm <| .get_get _
+      exact .refl _
+    | set s k ih =>
+      refine .trans ?_ <| .get_set _
+      refine .get ?_
+      intro s'
+      refine .trans ?_ <| .symm <| .set_set ..
+      clear s'
+      refine .trans ?_ <| ih.set s
+      clear ih
+      refine .trans ?_ <| .symm <| .set_get ..
+      refine .trans ?_ <| .symm <| .set_set ..
+      exact .refl _
+
+theorem StateM'.toStateM_get' : @toStateM σ σ MonadState.get = StateT.get := by simp [MonadState.get]; rfl
+theorem StateM'.toStateM_set' s : @toStateM σ PUnit (MonadState.set s) = StateT.set s := rfl
+
+theorem StateM'.toStateM_bind {β} (f : α → StateM' σ β) x : @toStateM σ β (bind f x) = StateT.bind (toStateM x) λ x => toStateM (f x) := by
+  funext s
+  induction x generalizing s with simp
+  | pure => rfl
+  | get _ ih => exact ih s s
+  | set s' _ ih => exact ih s'
+
+theorem StateM'.ofStateM_pure a : @ofStateM σ α (StateT.pure a) = pure a := by
+  apply Quot.sound
+  refine .trans ?_ <| .get_set _
+  refine .get ?_
+  intro s
+  apply Quotient.exact (s := ⟨_, _⟩)
+  exact Classical.choose_spec <| Quot.exists_rep _
+
+theorem StateM'.ofStateM_get' : @ofStateM σ σ StateT.get = MonadState.get := by
+  apply Quot.sound
+  apply FreeStateM.Eq.trans
+  . apply FreeStateM.Eq.get
+    intro s
+    apply Quotient.exact (s := ⟨_, _⟩)
+    exact Classical.choose_spec <| Quot.exists_rep _
+  . refine .symm ?_
+    apply FreeStateM.Eq.trans
+    . apply FreeStateM.Eq.get
+      intro s
+      apply Quotient.exact (s := ⟨_, _⟩)
+      exact Classical.choose_spec <| Quot.exists_rep _
+    . refine .trans (.symm <| .get_set _) ?_
+      apply FreeStateM.Eq.get
+      intro s
+      exact .set_get _ _
+
+theorem StateM'.ofStateM_set' s : @ofStateM σ PUnit (StateT.set s) = MonadState.set s := by
+  apply Quot.sound
+  apply FreeStateM.Eq.trans
+  . apply FreeStateM.Eq.get
+    intro s'
+    apply Quotient.exact (s := ⟨_, _⟩)
+    exact Classical.choose_spec <| Quot.exists_rep _
+  . refine .trans ?_ <| .get_set _
+    refine .get ?_
+    intro s'
+    refine .trans ?_ <| .symm <| .set_set ..
+    exact .refl _
+
+theorem StateM'.ofStateM_bind {β} (f : α → StateM σ β) x : @ofStateM σ β (StateT.bind x f) = bind (λ x => ofStateM (f x)) (ofStateM x) := by
+  apply Quot.sound
+  apply FreeStateM.Eq.trans
+  . apply FreeStateM.Eq.get
+    intro s
+    apply Quotient.exact (s := ⟨_, _⟩)
+    exact Classical.choose_spec <| Quot.exists_rep _
+  . refine .symm ?_
+    apply FreeStateM.Eq.trans
+    . apply FreeStateM.Eq.get
+      intro s
+      have : ∃ a, Quot.mk _ a = match x s with | (a, s) => Quot.mk FreeStateM.Eq (.set s <| .pure a) := Quot.exists_rep _
+      conv at «this» => rhs; ext; rhs; change Quot.mk FreeStateM.Eq <| .set (x s).snd <| .pure (x s).fst
+      show FreeStateM.Eq (Classical.choose (_ : ∃ a, Quot.mk _ a = bind' _ (Classical.choose this))) _
+      have := bind_wf (λ x => ofStateM (f x)) (Classical.choose this) (.set (x s).snd <| .pure (x s).fst) <| Quotient.exact (s := ⟨_, .refl, .symm, .trans⟩) <| Classical.choose_spec this
+      simp [this]
+      apply Quotient.exact (s := ⟨_, _⟩)
+      exact Classical.choose_spec <| Quot.exists_rep _
+    . refine .get ?_
+      intro s
+      refine .trans (.set_get ..) ?_
+      refine .trans ?_ <| .set_set (x s).snd _ _
+      refine .set _ ?_
+      apply Quotient.exact (s := ⟨_, _⟩)
+      exact Classical.choose_spec <| Quot.exists_rep _
